pulse/examples/dsls/mini_steel/Pulse.Checker.fsti
@@ -17,5 +17,6 @@ val check (f:RT.fstar_top_env)
           (t:term)
           (pre:pure_term)
           (pre_typing: tot_typing f g pre Tm_VProp)
+          (post_hint:option term)
   : T.Tac (c:pure_comp { C_ST? c ==> comp_pre c == pre } &
            src_typing f g t c)
